wip

Logic/Modal/Standard/PLoN/Semantics.lean
@@ -33,6 +33,20 @@ abbrev terminalFrame (α) : FiniteFrame α where
 
 abbrev FrameClass (α : Type*) := Set (PLoN.Frame α)
 
+abbrev FiniteFrameClass (α : Type*) := Set (PLoN.FiniteFrame α)
+
+
+abbrev FrameClass.restrictFinite (𝔽 : FrameClass α) : FiniteFrameClass α := { F | F.toFrame ∈ 𝔽 }
+
+lemma FrameClass.iff_mem_restrictFinite {𝔽 : FrameClass α} (h : F ∈ 𝔽) : (finite : Finite F.World) → ⟨F⟩ ∈ 𝔽.restrictFinite := by
+  simp_all [FrameClass.restrictFinite];
+
+@[simp]
+def FiniteFrameClass.toFrameClass (𝔽 : FiniteFrameClass α) : FrameClass α := { F | ∃ F', F' ∈ 𝔽 ∧ F'.toFrame = F }
+
+abbrev FrameClass.restrictFinite' (𝔽 : FrameClass α) : FrameClass α := 𝔽.restrictFinite.toFrameClass
+postfix:max "ꟳ" => FrameClass.restrictFinite'
+
 
 abbrev Valuation (F : PLoN.Frame α) (α : Type*) := F.World → α → Prop
 
@@ -43,7 +57,10 @@ structure Model (α) where
 abbrev Model.World (M : PLoN.Model α) := M.Frame.World
 instance : CoeSort (PLoN.Model α) (Type _) := ⟨Model.World⟩
 
+structure FiniteModel (α) extends Model α where
+  [World_finite : Finite World]
 
+abbrev FiniteModel.FiniteFrame (M : PLoN.FiniteModel α) : PLoN.FiniteFrame α := { toFrame := M.Frame, World_finite := M.World_finite }
 
 end PLoN
 
@@ -216,16 +233,26 @@ variable (F : Frame α)
 
 def SerialOnFormula (p : Formula α) : Prop := Serial (F.Rel' p)
 
-def SerialOnTheory (T : Theory α) : Prop := ∀ p ∈ T, F.SerialOnFormula p
+def SerialOnTheory (T : Theory α) : Prop := ∀ p ∈ □''⁻¹T, F.SerialOnFormula p
 
-protected def Serial : Prop := ∀ p, F.SerialOnFormula p
+protected def Serial : Prop := F.SerialOnTheory Set.univ
 
+/-
+lemma serialOnTheory_of_serial (hSerial : F.Serial) : F.SerialOnTheory T := by
+  intro q _;
+  exact hSerial q;
+-/
 
 def TransitiveOnFormula (p : Formula α) : Prop := ∀ {x y z : F.World}, x ≺[□p] y → y ≺[p] z → x ≺[p] z
 
-def TransitiveOnTheory (T : Theory α) : Prop := ∀ p ∈ T, F.SerialOnFormula p
+def TransitiveOnTheory (T : Theory α) : Prop := ∀ p ∈ □''⁻¹^[2]T, F.TransitiveOnFormula p
 
-protected def Transitive (F : Frame α) := ∀ p, F.TransitiveOnFormula p
+protected def Transitive (F : Frame α) := F.TransitiveOnTheory Set.univ
+
+/-
+lemma transitiveOnTheory_of_transitive (hTrans : F.Transitive) : F.TransitiveOnTheory T := by
+  intro q _; exact hTrans q;
+-/
 
 end Frame
 
@@ -249,13 +276,14 @@ abbrev TransitiveFrameClass (α) : PLoN.FrameClass α := { F | Frame.Transitive 
 
 lemma TransitiveFrameClass.nonempty : (TransitiveFrameClass.{_, 0} α).Nonempty := by
   use terminalFrame α;
-  simp [Frame.Transitive, Frame.TransitiveOnFormula];
+  simp [Frame.Transitive, Frame.TransitiveOnTheory, Frame.TransitiveOnFormula];
 
 
 abbrev SerialFrameClass (α) : PLoN.FrameClass α := { F | Frame.Serial F }
 
 lemma SerialFrameClass.nonempty : (SerialFrameClass.{_, 0} α).Nonempty := by
   use terminalFrame α;
+  simp [Frame.Serial, Frame.SerialOnTheory, Frame.SerialOnFormula];
   intro p x; use x;
 
 
@@ -263,7 +291,7 @@ abbrev TransitiveSerialFrameClass (α) : PLoN.FrameClass α := { F | F.Transitiv
 
 lemma TransitiveSerialFrameClass.nonempty : (TransitiveSerialFrameClass.{_, 0} α).Nonempty := by
   use terminalFrame α;
-  simp [Frame.Transitive, Frame.Serial, Frame.TransitiveOnFormula, Frame.SerialOnFormula];
+  simp [Frame.Transitive, Frame.TransitiveOnTheory, Frame.TransitiveOnFormula, Frame.Serial, Frame.SerialOnTheory, Frame.SerialOnFormula];
   intro p x; use x;
 
 
@@ -274,7 +302,7 @@ lemma N4_characterized : 𝐍𝟒.CharacterizedByPLoNFrameClass (TransitiveFrame
   induction hp using Deduction.inducition_with_necOnly! with
   | hMaxm h =>
     obtain ⟨p, e⟩ := h; subst e;
-    exact validAxiomFour_of_transitive (hTrans p);
+    exact validAxiomFour_of_transitive $ hTrans p (by simp_all);
   | hMdp ihpq ihp => exact PLoN.ValidOnFrame.mdp ihpq ihp;
   | hNec ihp => exact PLoN.ValidOnFrame.nec ihp;
   | hOrElim => exact PLoN.ValidOnFrame.disj₃;
@@ -292,7 +320,7 @@ lemma NRosser_characterized : 𝐍(𝐑).CharacterizedByPLoNFrameClass (SerialFr
     . obtain ⟨p, e⟩ := hNec; subst e; simp_all;
       exact PLoN.ValidOnFrame.nec ih;
     . obtain ⟨p, e⟩ := hRosser; subst e; simp_all;
-      exact validRosserRule_of_serial (hSerial _) ih;
+      exact validRosserRule_of_serial (hSerial p (by simp_all)) ih;
   | hOrElim => exact PLoN.ValidOnFrame.disj₃;
   | _ => simp_all [PLoN.Satisfies];
 
@@ -304,16 +332,17 @@ lemma N4Rosser_characterized : 𝐍𝟒(𝐑).CharacterizedByPLoNFrameClass (Tra
   induction hp using Deduction.inducition! with
   | hMaxm h =>
     obtain ⟨p, e⟩ := h; subst e;
-    exact validAxiomFour_of_transitive (hTrans p);
+    exact validAxiomFour_of_transitive $ hTrans p (by simp_all);
   | hMdp ihpq ihp => exact PLoN.ValidOnFrame.mdp ihpq ihp;
   | hRules rl hrl hant ih =>
     rcases hrl with (hNec | hRosser)
     . obtain ⟨p, e⟩ := hNec; subst e; simp_all;
       exact PLoN.ValidOnFrame.nec ih;
     . obtain ⟨p, e⟩ := hRosser; subst e; simp_all;
-      exact validRosserRule_of_serial (hSerial _) ih;
+      exact validRosserRule_of_serial (hSerial (□p) (by simp_all)) ih;
   | hOrElim => exact PLoN.ValidOnFrame.disj₃;
   | _ => simp_all [PLoN.Satisfies];
+
 
 end PLoN
 
